<?xml version="1.0" encoding="utf-8"?>
<rdf:RDF xmlns:daq="http://purl.org/eis/vocab/daq#"
   xmlns:dc="http://purl.org/dc/elements/1.1/"
   xmlns:dct="http://purl.org/dc/terms/"
   xmlns:foaf="http://xmlns.com/foaf/0.1/"
   xmlns:owl="http://www.w3.org/2002/07/owl#"
   xmlns:qpro="http://purl.org/eis/vocab/qpro#"
   xmlns:rdf="http://www.w3.org/1999/02/22-rdf-syntax-ns#"
   xmlns:rdfg="http://www.w3.org/2004/03/trix/rdfg-1"
   xmlns:rdfs="http://www.w3.org/2000/01/rdf-schema#"
   xmlns:voaf="http://purl.org/vocommons/voaf#"
   xmlns:xsd="http://www.w3.org/2001/XMLSchema#">
  <owl:Ontology rdf:about="http://purl.org/eis/vocab/qpro#">
    <dct:creator>
      <rdf:Description>
        <foaf:homepage rdf:resource="http://www.jeremydebattista.info"/>
        <foaf:mbox rdf:resource="mailto:debattis@cs.uni-bonn.de"/>
        <foaf:name>Jeremy Debattista</foaf:name>
      </rdf:Description>
    </dct:creator>
    <dct:modified rdf:datatype="http://www.w3.org/2001/XMLSchema#date">2015-04-01</dct:modified>
    <rdf:type rdf:resource="http://purl.org/vocommons/voaf#Vocabulary"/>
    <rdfs:comment>The Quality Problem Report (QPRO) enables the fine-grained description of quality problems found while assessing a dataset.</rdfs:comment>
    <rdfs:label>Quality Problem Report (QPRO)</rdfs:label>
  </owl:Ontology>
  <rdfs:Class rdf:about="http://purl.org/eis/vocab/qpro#Exception">
    <rdfs:comment>Represents an Exception that causes the dataset to have Quality Problems. This is an abstract class</rdfs:comment>
    <rdfs:label>Exception (Abstract)</rdfs:label>
  </rdfs:Class>
  <rdfs:Class rdf:about="http://purl.org/eis/vocab/qpro#QualityProblem">
    <rdfs:comment>Represents a quality problem detected during the assessment of quality metrics on triples.</rdfs:comment>
    <rdfs:label>Quality Problem</rdfs:label>
  </rdfs:Class>
  <rdfs:Class rdf:about="http://purl.org/eis/vocab/qpro#QualityReport">
    <rdfs:comment>Represents a report on the problems detected during the assessment of quality on a dataset.</rdfs:comment>
    <rdfs:label>Quality Report</rdfs:label>
  </rdfs:Class>
  <rdf:Property rdf:about="http://purl.org/eis/vocab/qpro#computedOn">
    <rdfs:comment>Represents the dataset URI on which quality metrics where computed</rdfs:comment>
    <rdfs:domain rdf:resource="http://purl.org/eis/vocab/qpro#QualityReport"/>
    <rdfs:label>computed on</rdfs:label>
    <rdfs:range rdf:resource="http://www.w3.org/2000/01/rdf-schema#Resource"/>
  </rdf:Property>
  <rdfs:Property rdf:about="http://purl.org/eis/vocab/qpro#exceptionDescription">
    <rdfs:comment>Describes a particular exception raised by the Resource or Triple in question, causing a quality problem</rdfs:comment>
    <rdfs:domain rdf:resource="http://www.w3.org/2000/01/rdf-schema#Resource"/>
    <rdfs:label>Exception Description</rdfs:label>
    <rdfs:range rdf:resource="http://purl.org/eis/vocab/qpro#Exception"/>
    <rdfs:range rdf:resource="http://www.w3.org/2001/XMLSchema#Literal"/>
  </rdfs:Property>
  <rdfs:Property rdf:about="http://purl.org/eis/vocab/qpro#extraExceptionProperty">
    <rdfs:comment>Enables the description of extra exception properties. This is an abstract property.</rdfs:comment>
    <rdfs:label>Extra Exception Property (Abstract)</rdfs:label>
  </rdfs:Property>
  <rdf:Property rdf:about="http://purl.org/eis/vocab/qpro#hasProblem">
    <rdfs:comment>Identifies problem instances in the report</rdfs:comment>
    <rdfs:domain rdf:resource="http://purl.org/eis/vocab/qpro#QualityReport"/>
    <rdfs:label>has problem</rdfs:label>
    <rdfs:range rdf:resource="http://purl.org/eis/vocab/qpro#QualityProblem"/>
  </rdf:Property>
  <rdf:Property rdf:about="http://purl.org/eis/vocab/qpro#inGraph">
    <rdfs:comment>This property enables the reification of quads by creating a new property to define the context of a triple statement.</rdfs:comment>
    <rdfs:domain rdf:resource="http://www.w3.org/1999/02/22-rdf-syntax-ns#Statement"/>
    <rdfs:label>in graph</rdfs:label>
    <rdfs:range rdf:resource="http://www.w3.org/2004/03/trix/rdfg-1Graph"/>
  </rdf:Property>
  <rdf:Property rdf:about="http://purl.org/eis/vocab/qpro#isDescribedBy">
    <rdfs:comment>Represent the URI of the metric which instantiated this problem</rdfs:comment>
    <rdfs:domain rdf:resource="http://purl.org/eis/vocab/qpro#QualityProblem"/>
    <rdfs:label>is described by</rdfs:label>
    <rdfs:range rdf:resource="http://purl.org/eis/vocab/daq#Metric"/>
  </rdf:Property>
  <rdf:Property rdf:about="http://purl.org/eis/vocab/qpro#problematicThing">
    <rdfs:comment>Represent the actual problematic instance from the dataset. This could be a list of resources (rdf:Seq), a list of reified statements, or a model representing a list of statements.</rdfs:comment>
    <rdfs:domain rdf:resource="http://purl.org/eis/vocab/qpro#QualityProblem"/>
    <rdfs:label>Problematic Thing</rdfs:label>
    <rdfs:range rdf:resource="http://www.w3.org/2000/01/rdf-schema#Resource"/>
  </rdf:Property>
</rdf:RDF>
