@prefix daq:     <http://purl.org/eis/vocab/daq#> .
@prefix dqm:     <http://www.diachron-fp7.eu/dqm#> .
@prefix owl:	 <http://www.w3.org/2002/07/owl#> .
@prefix rdf:     <http://www.w3.org/1999/02/22-rdf-syntax-ns#> .
@prefix rdfg:	 <http://www.w3.org/2004/03/trix/rdfg-1> .
@prefix rdfs:    <http://www.w3.org/2000/01/rdf-schema#> .
@prefix xsd:     <http://www.w3.org/2001/XMLSchema#> .
@prefix qpro:     <http://purl.org/eis/vocab/qpro#> .
@prefix prov: <http://www.w3.org/ns/prov#> .

##########################
# Provenance Information #
##########################

dqm:LuzzuProvenanceAgent
	a		prov:SoftwareAgent ;
	rdfs:label	"Luzzu Quality Assessment Framework"^^xsd:string .

####

	#Category Classes
	dqm:Accessibility
		a	rdfs:Class ;
		rdfs:subClassOf	daq:Category ;
		rdfs:comment	"Encompasses dimensions related to the ability to access to and retrieve the dataset required for a particular use case" ;
		rdfs:label	"Accessibility" .
		
	dqm:Intrinsic
		a	rdfs:Class ;
		rdfs:subClassOf	daq:Category ;
		rdfs:comment	"Refers to dimensions that are independent of the user's context and that measure the correctness, succinctness and consistency of the dataset" ;
		rdfs:label	"Intrinsic" .
		
	dqm:Trust
		a	rdfs:Class ;
		rdfs:subClassOf	daq:Category ;
		rdfs:comment	"Dimensions belonging to this group focus on the perceived trustworthiness of the dataset and its sources" ;
		rdfs:label	"Trust" .
		
	dqm:Dynamicity
		a	rdfs:Class ;
		rdfs:subClassOf	daq:Category ;
		rdfs:comment	"Dimensions in this category provide information about how current is the data (i.e. its freshness over time) and how frequently it changes" ;
		rdfs:label	"Dynamicity" .
	
	dqm:Contextual
		a	rdfs:Class ;
		rdfs:subClassOf	daq:Category ;
		rdfs:comment	"Comprises dimensions that highly depend on the context of the task to be performed" ;
		rdfs:label	"Contextual" .
		
	dqm:Representational
		a	rdfs:Class ;
		rdfs:subClassOf	daq:Category ;
		rdfs:comment	"Groups dimensions related to the design of the data, which provide information about how the chosen representation of the data affect its quality" ;
		rdfs:label	"Representational" .
	
	dqm:Reputation
		a	rdfs:Class ;
		rdfs:subClassOf	daq:Category ;
		rdfs:comment	"Reputation dimensions related to the reputation of the data, which provide information about how the reputable the data is based on its providers and host" ;
		rdfs:label	"Reputation" .
		
	#Dimension Classes
	dqm:Availability
		a	rdfs:Class ;
		rdfs:subClassOf	daq:Dimension ;
		rdfs:comment	"Metrics in this dimension measure the extent to which information (or some portion of it) is present, obtainable and ready for use" ;
		rdfs:label	"Availability" .
		
	dqm:Licensing
		a	rdfs:Class ;
		rdfs:subClassOf	daq:Dimension ;
		rdfs:comment	"Indicates whether consumers of the dataset are explicitly granted permissions to use it, under defined conditions (if any)" ;
		rdfs:label	"Licensing" .
		
	dqm:Security
		a	rdfs:Class ;
		rdfs:subClassOf	daq:Dimension ;
		rdfs:comment	"Refers to the extent to which data is protected against illegal alteration and it's authenticity can be guaranteed and to the confidentiality of the communication between a source and its consumers" ;
		rdfs:label	"Security" .
		
	dqm:Performance
		a	rdfs:Class ;
		rdfs:subClassOf	daq:Dimension ;
		rdfs:comment	"Assesses the efficiency with which a system can bind to the dataset and get access to the information contained into it" ;
		rdfs:label	"Performance" .
		
	dqm:Interlinking
		a rdfs:Class;
		rdfs:subClassOf	daq:Dimension ;
		rdfs:comment	"Refers to the degree to which entities that represent the same concept are linked to each other, be it within or between two or more data sources." ;
		rdfs:label	"Interlinking" .
		
	dqm:Accuracy
		a	rdfs:Class ;
		rdfs:subClassOf	daq:Dimension ;
		rdfs:comment	"Extent to which data is correct. The degree to which the dataset correctly represents the real world and how much it is free of syntax errors. Classified in: Syntactic accuracy (the degree to which data values are close to their definition domain) and Semantic accuracy (the degree to which data values correctly represent the actual real world values)" ;
		rdfs:label	"Accuracy" .
			
	dqm:AmountOfData
		a	rdfs:Class ;
		rdfs:subClassOf	daq:Dimension ;
		rdfs:comment	"Refers to how appropriate the quantity and volume of data is for the task at hand. The amount of data should be enough to approximate the true scenario precisely" ;
		rdfs:label	"Amount of data" .
	
	dqm:Consistency
		a	rdfs:Class ;
		rdfs:subClassOf	daq:Dimension ;
		rdfs:comment	"Consistency means that a knowledge base is free of (logical/formal) contradictions with respect to particular knowledge representation and inference mechanisms" ;
		rdfs:label	"Consistency" .
	
	dqm:Conciseness
		a	rdfs:Class ;
		rdfs:subClassOf	daq:Dimension ;
		rdfs:comment	"Refers to the redundancy of entities, be it at the schema or the data level" ;
		rdfs:label	"Conciseness" .
		
	dqm:RepresentationalConciseness
		a	rdfs:Class ;
		rdfs:subClassOf	daq:Dimension ;
		rdfs:comment	"Measures the extent to which the representation of data is compact, clear and well formatted" ;
		rdfs:label	"Representational conciseness" .
	
	dqm:Versatility
		a	rdfs:Class ;
		rdfs:subClassOf	daq:Dimension ;
		rdfs:comment	"Measures the availability of the data in different representations and in an internationalised way" ;
		rdfs:label	"Versatility" .

	dqm:Interpretability
		a	rdfs:Class ;
		rdfs:subClassOf	daq:Dimension ;
		rdfs:comment	"Refers to technical aspects of the data, that is, whether information is represented using an appropriate notation" ;
		rdfs:label	"Interpretability" .

	dqm:Interoperability
		a	rdfs:Class ;
		rdfs:subClassOf	daq:Dimension ;
		rdfs:comment	"Refers to the degree to which the format and structure of the information conforms to previously returned information as well as data from other sources." ;
		rdfs:label	"Interoperability" .
	
	dqm:Currency
		a	rdfs:Class ;
		rdfs:subClassOf	daq:Dimension ;
		rdfs:comment	"Provides a measure of the degree to which information is up to date and how promptly the data is updated" ;
		rdfs:label	"Currency" .
		
	dqm:Volatility
		a	rdfs:Class ;
		rdfs:subClassOf	daq:Dimension ;
		rdfs:comment	"Refers to the frequency with which data varies in time" ;
		rdfs:label	"Volatility" .
		
	dqm:Timeliness
		a	rdfs:Class ;
		rdfs:subClassOf	daq:Dimension ;
		rdfs:comment	"Indicates how up-to-date the data is, relative to the specific task at hand" ;
		rdfs:label	"Timeliness" .

	dqm:Understandability
		a	rdfs:Class ;
		rdfs:subClassOf	daq:Dimension ;
		rdfs:comment	"Refers to the easy with which data can be compreshended without ambiguity and used by a human data consumer" ;
		rdfs:label	"Understandability" .
		
	dqm:Provenance
		a	rdfs:Class ;
		rdfs:subClassOf daq:Dimension ;
		rdfs:comment "Refers to the dataset's representation of provenance information" ;
		rdfs:label "Provenance" .
			
	#Metric Classes
	dqm:EndPointAvailabilityMetric
		a	rdfs:Class ;
		rdfs:subClassOf	daq:Metric ; 
		daq:expectedDataType xsd:double ;
		rdfs:comment	"Checks whether the server (endpoint) is reachable and responds to a SPARQL query" ;
		rdfs:label	"Availability of the SPARQL end-point metric" .		

	dqm:RDFAvailabilityMetric
		a	rdfs:Class ;
		rdfs:subClassOf	daq:Metric ; 
		daq:expectedDataType xsd:double ;
		rdfs:comment	"Upon request of an RDF dump, checks whether it is provided as result" ;
		rdfs:label	"Availability of the RDF dumps metric" .	

	dqm:DereferenceabilityMetric
		a	rdfs:Class ;
		rdfs:subClassOf	daq:Metric ; 
		daq:expectedDataType xsd:double ;
		rdfs:comment	"Determines whether requesting a resource, identified by a URI, results in an error code being returned (e.g. 4xx: client error or 5xx: server error), or in a broken link" ;
		rdfs:label	"Dereferenceability metric" .	

	dqm:UnstructuredMetric
		a	rdfs:Class ;
		rdfs:subClassOf	daq:Metric ; 
		daq:expectedDataType xsd:double ;
		rdfs:comment	"Detects dead links or URIs without any supporting RDF metadata or no redirection using the status code 303" ;
		rdfs:label	"No structured data available metric" .			

	dqm:DereferenceabilityBackLinksMetric
		a	rdfs:Class ;
		rdfs:subClassOf	daq:Metric ; 
		daq:expectedDataType xsd:double ;
		rdfs:comment	"Detects all local in-links or back-links (locally available triples with the resource URI appearing as object, in the dereferenced document returned for the resource)" ;
		rdfs:label	"Dereferenceability of back-links metric" .	

	dqm:DereferenceabilityForwardLinksMetric
		a	rdfs:Class ;
		rdfs:subClassOf	daq:Metric ; 
		daq:expectedDataType xsd:double ;
		rdfs:comment	"Detects all forward links (locally known triples where the local URI is mentioned in the subject)" ;
		rdfs:label	"Dereferenceability of forward-links metric" .	

	dqm:MisreportedContentTypesMetric
		a	rdfs:Class ;
		rdfs:subClassOf	daq:Metric ; 
		daq:expectedDataType xsd:double ;
		rdfs:comment	"Checks whether the content is suitable for consumption and if such content should be accessed" ;
		rdfs:label	"Misreported content types metric" .	
		
	dqm:MachineReadableLicenseMetric
		a	rdfs:Class ;
		rdfs:subClassOf	daq:Metric ; 
		daq:expectedDataType xsd:double ;
		rdfs:comment	"Verifies that the resource is annotated with a machine-readable indication of the license (e.g. a VoID description or dcterms:license property)" ;
		rdfs:label	"Machine-readable indication of a license metric" .
		
	dqm:HumanReadableLicenseMetric
		a	rdfs:Class ;
		rdfs:subClassOf	daq:Metric ; 
		daq:expectedDataType xsd:double ;
		rdfs:comment	"Verifies whether a human-readable text, stating the licensing model attributed to the resource, has been provided as part of the dataset" ;
		rdfs:label	"Human-readable indication of a license metric" .
		
	dqm:IndicationOfAttributionCopyLeftMetric
		a	rdfs:Class ;
		rdfs:subClassOf	daq:Metric ; 
		daq:expectedDataType xsd:double ;
		rdfs:comment	"Detects whether the work is attributed by the author under a CopyLeft license, which guarantees that free access to the resource and any modified versions of it, will always be provided" ;
		rdfs:label	"Indication of Attribution CopyLeft" .

	dqm:LowLatencyMetric
		a	rdfs:Class ;
		rdfs:subClassOf	daq:Metric ; 
		daq:expectedDataType xsd:double ;
		rdfs:comment	"Measures the delay between the submission of a request to the data source and the reception of the respective response (or the first part of it)" ;
		rdfs:label	"Low latency metric" .
		
	dqm:HighThroughputMetric
		a	rdfs:Class ;
		rdfs:subClassOf	daq:Metric ; 
		daq:expectedDataType xsd:double ;
		rdfs:comment	"Measures the number of answered HTTP requests responsed by the source of the dataset, per second" ;
		rdfs:label	"High throughput metric" .
		
	dqm:ScalabilityOfDataSourceMetric
		a	rdfs:Class ;
		rdfs:subClassOf	daq:Metric ; 
		daq:expectedDataType xsd:double ;
		rdfs:comment	"Determines whether the time required to answer a set of N requests divided by N, is not longer than the time it takes to answer a single request" ;
		rdfs:label	"Scalability of a data source metric" .
		
	dqm:NoUsageOfSlashURIsMetric
		a	rdfs:Class ;
		rdfs:subClassOf	daq:Metric ; 
		daq:expectedDataType xsd:double ;
		rdfs:comment	"Determines whether the extent to which hash URIs are used instead of slash URIs, as the latter usually imply that 303 redirects must be performed to gather all the elements described in the dataset" ;
		rdfs:label	"No usage of slash URIs metric" .

	dqm:CorrectURIUsage
		a	rdfs:Class ;
		rdfs:subClassOf	daq:Metric ; 
		daq:expectedDataType xsd:double ;
		rdfs:comment	"Determines whether URIs in a dataset are represented as Slash URIs if dataset is large, or Hash URIs otherwise" ;
		rdfs:label	"Correct Usage of Cool URIs" .


	dqm:MalformedDatatypeLiteralsMetric
		a	rdfs:Class ;
		rdfs:subClassOf	daq:Metric ; 
		daq:expectedDataType xsd:double ;
		rdfs:comment	"Detects ill-typed literals, which do not abide by the lexical syntax of their respective datatypes" ;
		rdfs:label	"Malformed datatype literals metric" .		
	
	dqm:IncompatibleDatatypeRangeMetric
		a	rdfs:Class ;
		rdfs:subClassOf	daq:Metric ; 
		daq:expectedDataType xsd:double ;
		rdfs:comment	"Detects literals incompatible with range data type" ;
		rdfs:label	"Incompatible datatype range metric" .
	
	dqm:HomogeneousDatatypesMetric
		a	rdfs:Class ;
		rdfs:subClassOf	daq:Metric ; 
		daq:expectedDataType xsd:double ;
		rdfs:comment	"Detects outliers or conflicts of literal datatypes. Since it is meant to measure the homogeneity and not the validity possible rdfs:range restrictions are not evaluated" ;
		rdfs:label	"Homogeneous datatypes metric" .
	
	dqm:MisplacedClassesOrPropertiesMetric
		a	rdfs:Class ;
		rdfs:subClassOf	daq:Metric ; 
		daq:expectedDataType xsd:double ;
		rdfs:comment	"Find resources that are - defined as a property but also appear on subject or object positions in other triples (except cases like ex:prop rdf:type rdfs:Property, ex:prop rds:subPropetyOf) - defined as a class but also appear on predicate position in other triples. The metric is computed as a ratio of misplaced classes and properties" ;
		rdfs:label	"Misplaced classes or properties metric" .
	
	dqm:MisusedOwlDatatypeOrObjectPropertiesMetric
		a	rdfs:Class ;
		rdfs:subClassOf	daq:Metric ; 
		daq:expectedDataType xsd:double ;
		rdfs:comment	"Detect properties that are defined as a owl:datatype property but is used as object property and properties defined as a owl:object property and used as datatype property The metric is computed as a ratio of misused properties" ;
		rdfs:label	"Misuse Owl datatype or object properties metric" .
		
	dqm:UndefinedClassesAndPropertiesMetric
		a	rdfs:Class ;
		rdfs:subClassOf	daq:Metric ; 
		daq:expectedDataType xsd:double ;
		rdfs:comment	"Detects undefined classes and properties" ;
		rdfs:label	"Undefined classes and properties metric" .
		
		
	dqm:OntologyHijackingMetric
		a	rdfs:Class ;
		rdfs:subClassOf	daq:Metric ;
		daq:expectedDataType xsd:double ;
		rdfs:comment	"Detects the redefinition by third parties of external classes/properties such that reasoning over data using those external terms is affected" ;
		rdfs:label	"Ontology hijacking metric" .	
			
	dqm:AmountOfTriplesMetric
		a	rdfs:Class ;
		rdfs:subClassOf	daq:Metric ; 
		daq:expectedDataType xsd:double ;
		rdfs:comment	"Counts the total number of triples present in the dataset" ;
		rdfs:label	"Amount of triples metric" .

	dqm:EntitiesAsMembersOfDisjointClassesMetric
		a	rdfs:Class ;
		rdfs:subClassOf	daq:Metric ; 
		daq:expectedDataType xsd:double ;
		rdfs:comment	"the ratio of entities described as members of disjoint classes (here: classes explicitly known as disjoint) to the total number of entities described in the dataset" ;
		rdfs:label	"Entities as members of disjoint classes metric" .
		
	dqm:IntensionalConcisenessMetric
		a	rdfs:Class ;
		rdfs:subClassOf	daq:Metric ; 
		daq:expectedDataType xsd:double ;
		rdfs:comment	"Provides a measure of the redundancy of the dataset at the schema level, computed as the ratio of the Number of Unique Attributes (Properties) to the Total Number of Attributes in the target schema" ;
		rdfs:label	"Intensional conciseness metric" .
		
	dqm:ExtensionalConcisenessMetric
		a	rdfs:Class ;
		rdfs:subClassOf	daq:Metric ; 
		daq:expectedDataType xsd:double ;
		rdfs:comment	"Provides a measure of the redundancy of the dataset at the data level, computed as the ratio of the Number of Unique Subjects to the Total Number of Subjects" ;
		rdfs:label	"Extensional conciseness metric" .
		
	dqm:DuplicateInstanceMetric
		a	rdfs:Class ;
		rdfs:subClassOf	daq:Metric ; 
		daq:expectedDataType xsd:double ;
		rdfs:comment	"Provides a measure of the redundancy of entities at the data level (ratio of entities that violate the uniqueness rule)" ;
		rdfs:label	"Duplicate instance metric" .
		
	dqm:ShortURIsMetric
		a	rdfs:Class ;
		rdfs:subClassOf	daq:Metric ; 
		daq:expectedDataType xsd:double ;
		rdfs:comment	"Detects the use of short URIs (and the avoidance of query parameters), which suggests that information is compactly represented and favors readability" ;
		rdfs:label	"Short URIs metric" .

	dqm:NoProlixRDFMetric
		a	rdfs:Class ;
		rdfs:subClassOf	daq:Metric ; 
		daq:expectedDataType xsd:double ;
		rdfs:comment	"Detects the use of prolix RDF features, i.e reification statements, containers and collections" ;
		rdfs:label	"No Use of Prolix RDF features metric" .

	dqm:DifferentSerialisationsMetric
		a	rdfs:Class ;
		rdfs:subClassOf	daq:Metric ; 
		daq:expectedDataType xsd:double ;
		rdfs:comment	"Detects if a dataset has more than one serialisation format" ;
		rdfs:label	"Different Serialisation Metric" .

	dqm:MultipleLanguageUsageMetric
		a	rdfs:Class ;
		rdfs:subClassOf	daq:Metric ; 
		daq:expectedDataType xsd:double ;
		rdfs:comment	"Detects if a dataset has more than one language" ;
		rdfs:label	"Multiple Language Usage Metric" .


	dqm:NoBlankNodeMetric
		a	rdfs:Class ;
		rdfs:subClassOf	daq:Metric ; 
		daq:expectedDataType xsd:double ;
		rdfs:comment	"Provides a measure for the usage of blank nodes in a dataset" ;
		rdfs:label	"No blank node metric" .

	dqm:ReuseExistingTermsMetric
		a	rdfs:Class ;
		rdfs:subClassOf	daq:Metric ; 
		daq:expectedDataType xsd:double ;
		rdfs:comment	"Provides a qualitative measure for detecting the overlap of terms used in a dataset with existing terms." ;
		rdfs:label	"Reuse existing terms metric" .

	dqm:ReuseExistingVocabularyMetric
		a	rdfs:Class ;
		rdfs:subClassOf	daq:Metric ; 
		daq:expectedDataType xsd:double ;
		rdfs:comment	"Provides a qualitative measure for detecting the overlap of vocabularies used in a dataset." ;
		rdfs:label	"Reuse existing vocabularies metric" .
	
	dqm:CurrencyOfDatasetMetric
		a	rdfs:Class ;
		rdfs:subClassOf	daq:Metric ; 
		daq:expectedDataType xsd:double ;
		rdfs:comment	"Compares the time when the data was observed with the time when the data (document as a whole and individual triples) were last modified, thereby providing a measure of how current the dataset is" ;
		rdfs:label	"Currency of document/statements metric" .
	
	dqm:FreshnessOfDatasetMetric
		a	rdfs:Class ;
		rdfs:subClassOf	daq:Metric ; 
		daq:expectedDataType xsd:double ;
		rdfs:comment	"Checks if the data in the dataset is being updated with the original data" ;
		rdfs:label	"Freshness of Dataset Metric" .
	
	dqm:TimeSinceModificationMetric
		a	rdfs:Class ;
		rdfs:subClassOf	daq:Metric ; 
		daq:expectedDataType xsd:double ;
		rdfs:comment	"Provides a measure of the degree to which information is up to date, by comparing the current time with the time when the data was last modified" ;
		rdfs:label	"Time since modification metric" .
		
	dqm:ExclusionOfOutdatedDataMetric
		a	rdfs:Class ;
		rdfs:subClassOf	daq:Metric ; 
		daq:expectedDataType xsd:double ;
		rdfs:comment	"Provides a measure of the degree to which information is up to date, by comparing the total number of resources, described by the dataset, versus the number of those that are recognized to be outdated" ;
		rdfs:label	"Exclusion of outdated data metric" .
		
	dqm:TimeValidityIntervalMetric
		a	rdfs:Class ;
		rdfs:subClassOf	daq:Metric ; 
		daq:expectedDataType xsd:double ;
		rdfs:comment	"Measures the frequency with which data varies over time, by calculating the length of the time interval during which data remains valid." ;
		rdfs:label	"Time validity interval metric" .
		
	dqm:TimelinessOfResourceMetric
		a	rdfs:Class ;
		rdfs:subClassOf	daq:Metric ; 
		daq:expectedDataType xsd:double ;
		rdfs:comment	"Assesses the difference between the last modified time of the original data source and the last modified time of the semantic web source, thereby indicating if the resource is outdated" ;
		rdfs:label	"Timeliness of the resource metric" .
		
	dqm:HumanReadableLabellingMetric
		a	rdfs:Class ;
		rdfs:subClassOf	daq:Metric ; 
		daq:expectedDataType xsd:double ;
		rdfs:comment	"Assesses the percentage of entities having an rdfs:label or rdfs:comment" ;
		rdfs:label	"Human-readable labelling metric" .
	
	dqm:EmptyAnnotationValueMetric
		a	rdfs:Class ;
		rdfs:subClassOf	daq:Metric ; 
		daq:expectedDataType xsd:double ;
		rdfs:comment "EmptyAnnotationValue consider the following widely used annotation properties (labels, comments, notes, etc.) and identifies triples whose property is from a pre-configured list of annotation properties, and whose object is an empty string" ;
		rdfs:label "Empty annotation value metric" .
		
	dqm:LabelsUsingCapitalsMetric
		a	rdfs:Class ;
		rdfs:subClassOf	daq:Metric ; 
		daq:expectedDataType xsd:double ;
		rdfs:comment "Labels using capitals identifies triples whose property is from a pre-configured list of label properties, and whose object uses a bad style of capitalization" ;
		rdfs:label "Labels using capitals metric" .
		
	dqm:WhitespaceInAnnotationMetric
		a	rdfs:Class ;
		rdfs:subClassOf	daq:Metric ; 
		daq:expectedDataType xsd:double ;
		rdfs:comment "Whitespace in annotation consider the following widely used annotation properties (labels, comments, notes, etc.) and identifies triples whose property is from a pre-configured list of annotation properties, and whose object value has leading or ending white space in string." ; 
		rdfs:label "Whitespace in annotation metric" .
	
	dqm:ReputationOfDatasetMetric
		a	rdfs:Class ;
		rdfs:subClassOf	daq:Metric ; 
		daq:expectedDataType xsd:double ;
		rdfs:comment "Detects non reputable resources by retrieving URI of resources from data sets and comparing them with URI found in reputable resources." ; 
		rdfs:label "Reputation of dataset metric" .
		
	dqm:InterlinkDetectionMetric
		a	rdfs:Class ;
		rdfs:subClassOf	daq:Metric ; 
		daq:expectedDataType xsd:double ;
		rdfs:comment "This is a complex metric that detects good quality interlinks by measuring the (i) interlink degree; (ii) clustering coefficient; (iii) centrality; (iv) open sameAs chains; (v) sameAs description richness" ; 
		rdfs:label "Interlink Detection Metric" .
		
	dqm:LinksToExternalDataProvidersMetric
		a	rdfs:Class ;
		rdfs:subClassOf	daq:Metric ;
		daq:expectedDataType xsd:double ;
		rdfs:comment "Measures the degree to which the resource is linked to external data providers, that is, refers to the detection of links that connect the resource to external data provided by another data sources" ; 
		rdfs:label "Existence of links to external data providers" .
		
	dqm:ExtendedProvenanceMetric
		a	rdfs:Class ;
		rdfs:subClassOf	daq:Metric ;
		daq:expectedDataType xsd:double ;
		rdfs:comment "Measures the degree of the available provenance information (Agent and Datasource for Entities and Activities) that is available in a dataset for a consumer to get to know the origin of the datasource using the standard W3C Prov-O" ; 
		rdfs:label "Extended Provenance Metric" .
		
	dqm:BasicProvenanceMetric
		a	rdfs:Class ;
		rdfs:subClassOf	daq:Metric ;
		daq:expectedDataType xsd:double ;
		rdfs:comment "Measures the degree of the basic provenance information, i.e. the creator or publisher, of a datasource" ; 
		rdfs:label "Basic Provenance Metric" .
		
	#Properties
	#Accessibility Dimensions Properties
	dqm:hasAvailabilityDimension
		a	rdfs:Property ;	
		rdfs:subPropertyOf	daq:hasDimension ;
		rdfs:comment	"Links Accessibility Category with Availability Dimension" ;
		rdfs:label	"Accessibility has availability dimension" ;
		rdfs:domain	dqm:Accessibility ;
		rdfs:range	dqm:Availability .
		
	#Availability Metric Properties
	dqm:hasEndPointAvailabilityMetric
		a	rdfs:Property ;
		rdfs:subPropertyOf	daq:hasMetric ;
		rdfs:comment	"Links Availability Dimension with Endpoint Availability Metric (Endpoint Availability Metric belongs to the Availability Dimension)" ;
		rdfs:label	"Availability has end-point availability metric" ;
		rdfs:domain	dqm:Availability ;
		rdfs:range	dqm:EndPointAvailabilityMetric .

	dqm:hasRDFAvailabilityMetric
		a	rdfs:Property ;
		rdfs:subPropertyOf	daq:hasMetric ;
		rdfs:comment	"Links Availability Dimension with RDF Availability Metric (RDF Availability Metric belongs to the Availability Dimension)" ;
		rdfs:label	"Availability has RDF availability metric" ;
		rdfs:domain	dqm:Availability ;
		rdfs:range	dqm:RDFAvailabilityMetric .

	dqm:hasDereferenceabilityMetric
		a	rdfs:Property ;
		rdfs:subPropertyOf	daq:hasMetric ;
		rdfs:comment	"Links Availability Dimension with Dereferenceability Metric (Dereferenceability Metric belongs to the Availability Dimension)" ;
		rdfs:label	"Availability has dereferenceability metric" ;
		rdfs:domain	dqm:Availability ;
		rdfs:range	dqm:DereferenceabilityMetric .

	dqm:hasUnstructuredMetric
		a	rdfs:Property ;
		rdfs:subPropertyOf	daq:hasMetric ;
		rdfs:comment	"Links Availability Dimension with Unstructured Data Metric (Unstructured Data Metric belongs to the Availability Dimension)" ;
		rdfs:label	"Availability has no structured data available metric" ;
		rdfs:domain	dqm:Availability ;
		rdfs:range	dqm:UnstructuredMetric .		

	dqm:hasDereferenceabilityBackLinksMetric
		a	rdfs:Property ;
		rdfs:subPropertyOf	daq:hasMetric ;
		rdfs:comment	"Links Availability Dimension with Dereferenceability of Back-links Metric (Dereferenceability of Back-links Metric belongs to the Availability Dimension)" ;
		rdfs:label	"Availability has Dereferenceability of back-links metric" ;
		rdfs:domain	dqm:Interlinking ;
		rdfs:range	dqm:DereferenceabilityBackLinksMetric .

	dqm:hasDereferenceabilityForwardLinksMetric
		a	rdfs:Property ;
		rdfs:subPropertyOf	daq:hasMetric ;
		rdfs:comment	"Links Availability Dimension with Dereferenceability of Forward-links Metric (Dereferenceability of Forward-links Metric belongs to the Availability Dimension)" ;
		rdfs:label	"Availability has Dereferenceability of forward-links metric" ;
		rdfs:domain	dqm:Availability ;
		rdfs:range	dqm:DereferenceabilityForwardLinksMetric .

	dqm:hasMisreportedContentTypesMetric
		a	rdfs:Property ;
		rdfs:subPropertyOf	daq:hasMetric ;
		rdfs:comment	"Links Availability Dimension with Misreported Content Types Metric (Misreported Content Types Metric belongs to the Availability Dimension)" ;
		rdfs:label	"Availability has misreported content types metric" ;
		rdfs:domain	dqm:Availability ;
		rdfs:range	dqm:MisreportedContentTypesMetric .
		
	#Licensing Dimensions Properties
	dqm:hasLicensingDimension
		a	rdfs:Property ;	
		rdfs:subPropertyOf	daq:hasDimension ;
		rdfs:comment	"Links Accessibility Category with Licensing Dimension" ;
		rdfs:label	"Accessibility has licensing dimension" ;
		rdfs:domain	dqm:Accessibility ;
		rdfs:range	dqm:Licensing .
		
	dqm:hasMachineReadableLicenseMetric
		a	rdfs:Property ;
		rdfs:subPropertyOf	daq:hasMetric ;
		rdfs:comment	"Links Licensing Dimension with Machine-readable Indication of a License Metric (Machine-readable Indication of a License Metric belongs to the Licensing Dimension)" ;
		rdfs:label	"Licensing has machine-readable indication of a license metric" ;
		rdfs:domain	dqm:Licensing ;
		rdfs:range	dqm:MachineReadableLicenseMetric .
		
	dqm:hasHumanReadableLicenseMetric
		a	rdfs:Property ;
		rdfs:subPropertyOf	daq:hasMetric ;
		rdfs:comment	"Links Licensing Dimension with Human-readable Indication of a License Metric (Human-readable Indication of a License Metric belongs to the Licensing Dimension)" ;
		rdfs:label	"Licensing has human-readable indication of a license metric" ;
		rdfs:domain	dqm:Licensing ;
		rdfs:range	dqm:HumanReadableLicenseMetric .
		
	dqm:hasIndicationOfAttributionCopyLeftMetric
		a	rdfs:Property ;
		rdfs:subPropertyOf	daq:hasMetric ;
		rdfs:comment	"Links Licensing Dimension with Indication of Attribution CopyLeft Metric (Indication of Attribution CopyLeft Metric belongs to the Licensing Dimension)" ;
		rdfs:label	"Licensing has indication of attribution CopyLeft metric" ;
		rdfs:domain	dqm:Licensing ;
		rdfs:range	dqm:IndicationOfAttributionCopyLeftMetric .
		
	#Security Dimension Properties
	dqm:hasSecurityDimension
		a	rdfs:Property ;	
		rdfs:subPropertyOf	daq:hasDimension ;
		rdfs:comment	"Links Accessibility Category with Security Dimension" ;
		rdfs:label	"Accessibility has security dimension" ;
		rdfs:domain	dqm:Accessibility ;
		rdfs:range	dqm:Security .
	
	#Performance Dimension Properties
	dqm:hasPerformanceDimension
		a	rdfs:Property ;	
		rdfs:subPropertyOf	daq:hasDimension ;
		rdfs:comment	"Links Accessibility Category with Performance Dimension" ;
		rdfs:label	"Accessibility has performance dimension" ;
		rdfs:domain	dqm:Accessibility ;
		rdfs:range	dqm:Performance .
		
	dqm:hasLowLatencyMetric
		a	rdfs:Property ;
		rdfs:subPropertyOf	daq:hasMetric ;
		rdfs:comment	"Links the Performance Dimension with Low Latency Metric (Low Latency Metric belongs to the Performance Dimension)" ;
		rdfs:label	"Performance has low latency metric" ;
		rdfs:domain	dqm:Performance ;
		rdfs:range	dqm:LowLatencyMetric .
		
	dqm:hasHighThroughputMetric
		a	rdfs:Property ;
		rdfs:subPropertyOf	daq:hasMetric ;
		rdfs:comment	"Links Performance Dimension with High Throughput Metric (High Throughput Metric belongs to the Performance Dimension)" ;
		rdfs:label	"Performance has high throughput metric" ;
		rdfs:domain	dqm:Performance ;
		rdfs:range	dqm:HighThroughputMetric .
		
	dqm:hasScalabilityOfDataSourceMetric
		a	rdfs:Property ;
		rdfs:subPropertyOf	daq:hasMetric ;
		rdfs:comment	"Links Performance Dimension with Scalability of a Data Source Metric (Scalability of a Data Source Metric belongs to the Performance Dimension)" ;
		rdfs:label	"Performance has scalability of a data source metric" ;
		rdfs:domain	dqm:Performance ;
		rdfs:range	dqm:ScalabilityOfDataSourceMetric .
		
	dqm:hasNoUsageOfSlashURIsMetric
		a	rdfs:Property ;
		rdfs:subPropertyOf	daq:hasMetric ;
		rdfs:comment	"Links Performance Dimension with No Usage of Slash URIs Metric (No Usage of Slash URIs Metric belongs to the Performance Dimension)" ;
		rdfs:label	"Performance has no usage of slash URIs metric" ;
		rdfs:domain	dqm:Performance ;
		rdfs:range	dqm:NoUsageOfSlashURIsMetric .
	
	dqm:hasCorrectURIUsage
		a	rdfs:Property ;
		rdfs:subPropertyOf	daq:hasMetric ;
		rdfs:comment	"Links Performance Dimension with the Correct URI Usage Metric (Correct URI Usage Metric belongs to the Performance Dimension)" ;
		rdfs:label	"has Correct URI Usage" ;
		rdfs:domain	dqm:Performance ;
		rdfs:range	dqm:CorrectURIUsage .
	
		#Interlink Dimensions Properties
		dqm:hasInterlinkDimension
			a	rdfs:Property ;	
			rdfs:subPropertyOf	daq:hasDimension ;
			rdfs:comment	"Links Accessibility Category with Interlink Dimension" ;
			rdfs:label	"has interlink dimension" ;
			rdfs:domain	dqm:Accessibility ;
			rdfs:range	dqm:Interlinking .
		
		#Availability Metric Properties
		dqm:hasInterlinkDetectionMetricMetric
			a	rdfs:Property ;
			rdfs:subPropertyOf	daq:hasMetric ;
			rdfs:comment	"" ;
			rdfs:label	"has Interlink Detection Metric" ;
			rdfs:domain	dqm:Interlinking ;
			rdfs:range	dqm:InterlinkDetectionMetric .
			
	dqm:hasLinkToExternalDataProvidersMetric
		a	rdfs:Property ;
		rdfs:subPropertyOf	daq:hasMetric ;
		rdfs:comment	"Links the Interlinking Dimension with Existence of Links to External Data Providers Metric (Existence of Links to External Data Providers Metric belongs to the Interlinking Dimension)" ;
		rdfs:label	"Interlink has existence of links to external data providers metric" ;
		rdfs:domain	dqm:Interlinking ;
		rdfs:range	dqm:LinksToExternalDataProvidersMetric .

	#Accuracy Dimensions Properties
	dqm:hasAccuracyDimension
		a	rdfs:Property ;
		rdfs:subPropertyOf	daq:hasDimension ;
		rdfs:comment	"Links Intrinsic Category with Accuracy Dimension" ;
		rdfs:label	"Intrinsic has accuracy dimension" ;
		rdfs:domain	dqm:Intrinsic ;
		rdfs:range	dqm:Accuracy .
		
	dqm:hasMalformedDatatypeLiteralsMetric
		a	rdfs:Property ;
		rdfs:subPropertyOf	daq:hasMetric ;
		rdfs:comment	"Links Accuracy Dimension with Malformed Data Type Literals Metric (Malformed Data Type Literals Metric belongs to the Accuracy Dimension)" ;
		rdfs:label	"Accuracy has malformed data type literals metric" ;
		rdfs:domain	dqm:Accuracy ;
		rdfs:range	dqm:MalformedDatatypeLiteralsMetric .
		
	dqm:hasIncompatibleDatatypeRangeMetric
		a	rdfs:Property ;
		rdfs:subPropertyOf	daq:hasMetric ;
		rdfs:comment	"Links Accuracy Dimension with Incompatible Datatype Range Metric" ;
		rdfs:label	"hasIncompatibleDatatypeRangeMetric" ;
		rdfs:domain	dqm:Accuracy ;
		rdfs:range	dqm:IncompatibleDatatypeRangeMetric .
		
		
	#Consistency Dimensions Properties
	dqm:hasHomogeneousDatatypesMetric
		a	rdfs:Property ;
		rdfs:subPropertyOf	daq:hasMetric ;
		rdfs:comment	"Links Consistency Dimension with Homogeneous data types Metric" ;
		rdfs:label	"hasHomogeneousDatatypesMetric" ;
		rdfs:domain	dqm:Consistency ;
		rdfs:range	dqm:HomogeneousDatatypesMetric .
				
		
	dqm:hasMisusedOwlDatatypeOrObjectPropertiesMetric
		a	rdfs:Property ;
		rdfs:subPropertyOf	daq:hasMetric ;
		rdfs:comment	"Links Consistency Dimension with Misuse Owl- datatype or object properties metric" ;
		rdfs:label	"hasMisuseOwlDatatypeOrObjectPropertiesMetric" ;
		rdfs:domain	dqm:Consistency ;
		rdfs:range	dqm:MisusedOwlDatatypeOrObjectPropertiesMetric .
		
	dqm:hasMisplacedClassesOrPropertiesMetric
		a	rdfs:Property ;
		rdfs:subPropertyOf	daq:hasMetric ;
		rdfs:comment	"Links Consistency Dimension with misplaced classes or properties metric" ;
		rdfs:label	"hasMisplacedClassesOrPropertiesMetric" ;
		rdfs:domain	dqm:Consistency ;
		rdfs:range	dqm:MisplacedClassesOrPropertiesMetric .
		

	#Contextual Dimensions Properties
	dqm:hasAmountOfDataDimension
		a	rdfs:Property ;
		rdfs:subPropertyOf	daq:hasDimension ;
		rdfs:comment	"Links Contextual Category with Amount of Data Dimension" ;
		rdfs:label	"Contextual has amount of data dimension" ;
		rdfs:domain	dqm:Contextual ;
		rdfs:range	dqm:AmountOfData .
		
	dqm:hasAmountOfTriplesMetric
		a	rdfs:Property ;
		rdfs:subPropertyOf	daq:hasMetric ;
		rdfs:comment	"Links Amount of Data Dimension with Amount of Triples Metric (Amount of Triples Metric belongs to the Amount of Data Dimension)" ;
		rdfs:label	"Amount of Data has amount of triples metric" ;
		rdfs:domain	dqm:AmountOfData ;
		rdfs:range	dqm:AmountOfTriplesMetric .	

	#Consistency Dimensions Properties
	dqm:hasConsistencyDimension
		a rdfs:Property ;
		rdfs:subPropertyOf daq:hasDimension ;
		rdfs:comment "Links Intrinsic Category with Consistency Dimension" ;
		rdfs:label "Intrinsic has consistency dimension" ;
		rdfs:domain dqm:Intrinsic ;
		rdfs:range dqm:Consistency .
	
	dqm:hasEntitiesAsMembersOfDisjointClassesMetric
		a	rdfs:Property ;
		rdfs:subPropertyOf	daq:hasMetric ;
		rdfs:comment	"Links Consistency Dimension with ‘entities as members of disjoint classes’ Metric (Entities as Members of Disjoint Classes Metric belongs to the Consistency Dimension)" ;
		rdfs:label	"Consistency has entities as members of disjoint classes metric" ;
		rdfs:domain	dqm:Consistency ;
		rdfs:range	dqm:EntitiesAsMembersOfDisjointClassesMetric .	
		
	#Conciseness Dimensions Properties
	dqm:hasConcisenessDimension
		a rdfs:Property ;
		rdfs:subPropertyOf daq:hasDimension ;
		rdfs:comment "Links Intrinsic Category with Conciseness Dimension" ;
		rdfs:label "Intrinsic has conciseness dimension" ;
		rdfs:domain dqm:Intrinsic ;
		rdfs:range dqm:Conciseness .
	
	dqm:hasIntensionalConcisenessMetric
		a	rdfs:Property ;
		rdfs:subPropertyOf	daq:hasMetric ;
		rdfs:comment	"Links Conciseness Dimension with Intensional Conciseness Metric (Intensional Conciseness Metric belongs to the Conciseness Dimension)" ;
		rdfs:label	"Conciseness has intensional conciseness metric" ;
		rdfs:domain	dqm:Conciseness ;
		rdfs:range	dqm:IntensionalConcisenessMetric .	
		
	dqm:hasExtensionalConcisenessMetric
		a	rdfs:Property ;
		rdfs:subPropertyOf	daq:hasMetric ;
		rdfs:comment	"Links Conciseness Dimension with Extensional Conciseness Metric (Extensional Conciseness Metric belongs to the Conciseness Dimension)" ;
		rdfs:label	"Conciseness has extensional conciseness metric" ;
		rdfs:domain	dqm:Conciseness ;
		rdfs:range	dqm:ExtensionalConcisenessMetric .	
		
	dqm:hasDuplicateInstanceMetric
		a	rdfs:Property ;
		rdfs:subPropertyOf	daq:hasMetric ;
		rdfs:comment	"Links Conciseness Dimension with Duplicate Instance Metric (Duplicate Instance Metric belongs to the Conciseness Dimension)" ;
		rdfs:label	"Conciseness has duplicate instance metric" ;
		rdfs:domain	dqm:Conciseness ;
		rdfs:range	dqm:DuplicateInstanceMetric .
		
	#Representational Conciseness Dimension Properties
	dqm:hasRepresentationalConcisenessDimension
		a rdfs:Property ;
		rdfs:subPropertyOf daq:hasDimension ;
		rdfs:comment "Links Representational Category with Representational-Conciseness Dimension" ;
		rdfs:label "Representational has representational conciseness dimension" ;
		rdfs:domain dqm:Representational ;
		rdfs:range dqm:RepresentationalConciseness .
		
	dqm:hasShortURIsMetric
		a	rdfs:Property ;
		rdfs:subPropertyOf	daq:hasMetric ;
		rdfs:comment	"Links Representational-Conciseness Dimension with Keeping URIs Short Metric (Keeping URIs Short Metric belongs to the Representational-Conciseness Dimension)" ;
		rdfs:label	"Representational conciseness has short URIs metric" ;
		rdfs:domain	dqm:RepresentationalConciseness ;
		rdfs:range	dqm:ShortURIsMetric .
	
		
	dqm:hasNoProlixRDFMetric
		a	rdfs:Property ;
		rdfs:subPropertyOf	daq:hasMetric ;
		rdfs:comment	"Links Representational-Conciseness Dimension with No Usage of Prolix RDF features metric";
		rdfs:label	"Representational conciseness has no usage of prolix RDF features metric" ;
		rdfs:domain	dqm:RepresentationalConciseness ;
		rdfs:range	dqm:NoProlixRDFMetric .
		
	#Provenance Dimension Properties
	dqm:hasProvenanceDimension
		a rdfs:Property ;
		rdfs:subPropertyOf daq:hasDimension ;
		rdfs:domain dqm:Representational ;
		rdfs:range dqm:Provenance .
		
	dqm:hasBasicProvenanceMetric
		a	rdfs:Property ;
		rdfs:subPropertyOf	daq:hasMetric ;
		rdfs:domain	dqm:Provenance ;
		rdfs:range	dqm:BasicProvenanceMetric .
		
	dqm:hasExtendedProvenanceMetric
		a	rdfs:Property ;
		rdfs:subPropertyOf	daq:hasMetric ;
		rdfs:domain	dqm:Provenance ;
		rdfs:range	dqm:ExtendedProvenanceMetric .
	

	#Versatility Dimension Properties
	dqm:hasVersatilityDimension
		a rdfs:Property ;
		rdfs:subPropertyOf daq:hasDimension ;
		rdfs:comment "Links Representational Category with Versatility Dimension" ;
		rdfs:label "Representational has versatility dimension" ;
		rdfs:domain dqm:Representational ;
		rdfs:range dqm:Versatility .

	dqm:hasDifferentSerialisationsMetric
		a	rdfs:Property ;
		rdfs:subPropertyOf	daq:hasMetric ;
		rdfs:comment	"Links Versatility Dimension with Different Serialisations metric";
		rdfs:label	"Versatility has different serialisation metric " ;
		rdfs:domain	dqm:Versatility ;
		rdfs:range	dqm:DifferentSerialisationsMetric .


	dqm:hasMultipleLanguageUsageMetric
		a	rdfs:Property ;
		rdfs:subPropertyOf	daq:hasMetric ;
		rdfs:comment	"Links Versatility Dimension with Multiple Language Usage Metric";
		rdfs:label	"Versatility has multiple language usage " ;
		rdfs:domain	dqm:Versatility ;
		rdfs:range	dqm:MultipleLanguageUsageMetric .


	#Interpretability Dimension Properties
	dqm:hasInterpretabilityDimension
		a rdfs:Property ;
		rdfs:subPropertyOf daq:hasDimension ;
		rdfs:comment "Links Representational Category with Interpretability Dimension" ;
		rdfs:label "Representational has interpretability dimension" ;
		rdfs:domain dqm:Representational ;
		rdfs:range dqm:Interpretability .

	dqm:hasNoBlankNodeMetric
		a	rdfs:Property ;
		rdfs:subPropertyOf	daq:hasMetric ;
		rdfs:comment	"Links Interpretability Dimension with No Blank Node metric";
		rdfs:label	"Versatility has no blank node metric " ;
		rdfs:domain	dqm:Interpretability ;
		rdfs:range	dqm:NoBlankNodeMetric .

	dqm:hasUndefinedClassesAndPropertiesMetric
		a	rdfs:Property ;
		rdfs:subPropertyOf	daq:hasMetric ;
		rdfs:comment	"Links Consistency Dimension with Undefined classes and properties metric" ;
		rdfs:label	"hasUndefinedClassesMetric" ;
		rdfs:domain	dqm:Interpretability ;
		rdfs:range	dqm:UndefinedClassesAndPropertiesMetric .

	#Interoperability Dimension Properties
	dqm:hasInteroperabilityDimension
		a rdfs:Property ;
		rdfs:subPropertyOf daq:hasDimension ;
		rdfs:comment "Links Representational Category with Interoperability Dimension" ;
		rdfs:label "Representational has interoperability dimension" ;
		rdfs:domain dqm:Representational ;
		rdfs:range dqm:Interoperability .

	dqm:hasReuseExistingTermsMetric
		a	rdfs:Property ;
		rdfs:subPropertyOf	daq:hasMetric ;
		rdfs:comment	"Links Interoperability Dimension with Reuse Existing Terms";
		rdfs:label	"Interoperability has reuse existing terms metric " ;
		rdfs:domain	dqm:Interoperability ;
		rdfs:range	dqm:ReuseExistingTermsMetric .


	dqm:hasReuseExistingVocabularyMetric
		a	rdfs:Property ;
		rdfs:subPropertyOf	daq:hasMetric ;
		rdfs:comment	"Links Interoperability Dimension with reuse existing vocabulary metric";
		rdfs:label	"Interoperability has reuse existing vocabularies metric " ;
		rdfs:domain	dqm:Interoperability ;
		rdfs:range	dqm:ReuseExistingVocabularyMetric .



	
	#Understandability Dimension Properties
	dqm:hasRepresentationalConcisenessDimension
		a rdfs:Property ;
		rdfs:subPropertyOf daq:hasDimension ;
		rdfs:comment "Links Representational Category with Understandability Dimension" ;
		rdfs:label "Representational has representational conciseness dimension" ;
		rdfs:domain dqm:Representational ;
		rdfs:range dqm:Understandability .
		
	dqm:hasHumanReadableLabellingMetric
		a	rdfs:Property ;
		rdfs:subPropertyOf	daq:hasMetric ;
		rdfs:comment	"Links Understandability Dimension with Human Readable Labelling Metric (Human Readable Labelling belongs to the Understandability Dimension)" ;
		rdfs:label	"Understandability has short URIs metric" ;
		rdfs:domain	dqm:Understandability ;
		rdfs:range	dqm:HumanReadableLabellingMetric .
	
	dqm:hasEmptyAnnotationValueMetric
		a	rdfs:Property ;
		rdfs:subPropertyOf	daq:hasMetric ;
		rdfs:comment "Links Understandability Dimension with Empty annotation value metric" ;
		rdfs:label "Understandability has empty annotation value metric" ;
		rdfs:domain	dqm:Understandability ;
		rdfs:range	dqm:EmptyAnnotationValueMetric .
	
	dqm:hasLabelsUsingCapitalsMetric
		a	rdfs:Property ;
		rdfs:subPropertyOf	daq:hasMetric ;
		rdfs:comment "Links Understandability Dimension with labels using capitals metric" ;
		rdfs:label "Understandability has labels using capitals metric" ;
		rdfs:domain	dqm:Understandability ;
		rdfs:range	dqm:LabelsUsingCapitalsMetric .
		
	dqm:hasWhitespaceInAnnotationMetric
		a	rdfs:Property ;
		rdfs:subPropertyOf	daq:hasMetric ;
		rdfs:comment "Links Understandability Dimension with Whitespace in annotation" ;
		rdfs:label "Understandability has whitespace in annotation" ;
		rdfs:domain	dqm:Understandability ;
		rdfs:range	dqm:WhitespaceInAnnotationMetric .
				
	#Currency Dimension Properties
	dqm:hasCurrencyDimension
		a rdfs:Property ;
		rdfs:subPropertyOf daq:hasDimension ;
		rdfs:comment "Links the Dynamicity Category with the Currency Dimension" ;
		rdfs:label "Dynamicity has currency dimension" ;
		rdfs:domain dqm:Dynamicity ;
		rdfs:range dqm:Currency .

	dqm:hasCurrencyOfDatasetMetric
		a	rdfs:Property ;
		rdfs:subPropertyOf	daq:hasMetric ;
		rdfs:comment	"Links the Currency Dimension with the Currency of Document/Statements Metric (Currency of Document/Statements Metric belongs to the Currency Dimension)" ;
		rdfs:label	"Currency has currency of document/statements metric" ;
		rdfs:domain	dqm:Currency ;
		rdfs:range	dqm:CurrencyOfDatasetMetric .

	dqm:hasTimeSinceModificationMetric
		a	rdfs:Property ;
		rdfs:subPropertyOf	daq:hasMetric ;
		rdfs:comment	"Links the Currency Dimension with the Time Since Modification Metric (Time Since Modification Metric belongs to the Currency Dimension)" ;
		rdfs:label	"Currency has time since modification metric" ;
		rdfs:domain	dqm:Currency ;
		rdfs:range	dqm:TimeSinceModificationMetric .

	dqm:hasExclusionOfOutdatedDataMetric
		a	rdfs:Property ;
		rdfs:subPropertyOf	daq:hasMetric ;
		rdfs:comment	"Links the Currency Dimension with the Exclusion of Outdated Data Metric (Exclusion of Outdated Data Metric belongs to the Currency Dimension)" ;
		rdfs:label	"Currency has exclusion of outdated data metric" ;
		rdfs:domain	dqm:Currency ;
		rdfs:range	dqm:ExclusionOfOutdatedDataMetric .

	#Volatility Dimension Properties
	dqm:hasVolatilityDimension
		a rdfs:Property ;
		rdfs:subPropertyOf daq:hasDimension ;
		rdfs:comment "Links the Dynamicity Category with the Volatility Dimension" ;
		rdfs:label "Dynamicity has volatility dimension" ;
		rdfs:domain dqm:Dynamicity ;
		rdfs:range dqm:Volatility .

	dqm:hasTimeValidityIntervalMetric
		a	rdfs:Property ;
		rdfs:subPropertyOf	daq:hasMetric ;
		rdfs:comment	"Links the Volatility Dimension with the Time Validity Interval Metric (Time Validity Interval Metric belongs to the Volatility Dimension)" ;
		rdfs:label	"Volatility has time validity interval metric" ;
		rdfs:domain	dqm:Volatility ;
		rdfs:range	dqm:TimeValidityIntervalMetric .
		
	#Timeliness Dimension Properties
	dqm:hasTimelinessDimension
		a rdfs:Property ;
		rdfs:subPropertyOf daq:hasDimension ;
		rdfs:comment "Links the Dynamicity Category with the Timeliness Dimension" ;
		rdfs:label "Dynamicity has timeliness dimension" ;
		rdfs:domain dqm:Dynamicity ;
		rdfs:range dqm:Timeliness .
		
	dqm:hasTimelinessOfResourceMetric
		a	rdfs:Property ;
		rdfs:subPropertyOf	daq:hasMetric ;
		rdfs:comment	"Links the Timeliness Dimension with the Timeliness of the Resource Metric (Timeliness of the Resource Metric belongs to the Timeliness Dimension)" ;
		rdfs:label	"Timeliness has timeliness of resource metric" ;
		rdfs:domain	dqm:Timeliness ;
		rdfs:range	dqm:TimelinessOfResourceMetric .

	dqm:hasFreshnessOfDatasetMetric
		a	rdfs:Property ;
		rdfs:subPropertyOf	daq:hasMetric ;
		rdfs:domain	dqm:Timeliness ;
		rdfs:range	dqm:FreshnessOfDatasetMetric .

		
	#Reputation
	dqm:hasReputationOfDatasetMetric
		a	rdfs:Property ;
		rdfs:subPropertyOf	daq:hasMetric ;
		rdfs:comment "Links Reputation category with Reputation of dataset metric" ; 
		rdfs:label "Reputation category has reputation of dataset metric" ;
		rdfs:domain	dqm:Reputation ;
		rdfs:range	dqm:ReputationOfDatasetMetric .
			
##################################
#				 #
#	EBI SPECIFIC METRICS	 #
#				 #
##################################

#Ontology Versioning Conciseness
dqm:hasOntologyVersionConcisenessMetric
	a	rdfs:Property ;
	rdfs:subPropertyOf	daq:hasMetric ;
	rdfs:comment	"Links Conciseness Dimension with Ontology Versioning Conciseness Metric" ;
	rdfs:label	"Conciseness has extensional conciseness metric" ;
	rdfs:domain	dqm:Conciseness ;
	rdfs:range	dqm:OntologyVersionConcisenessMetric .	
	
dqm:OntologyVersionConcisenessMetric
		a	rdfs:Class ;
		rdfs:subClassOf	daq:Metric ; 
		daq:expectedDataType xsd:double ;
		rdfs:comment	"Provides a measure for checking singleton instances of the use-case specific defined owl:ontologyVersion property" ;
		rdfs:label	"Ontology version conciseness metric" .
		
		
#Obsolete Concepts in Ontology
dqm:hasObsoleteConceptsInOntologyMetric
	a	rdfs:Property ;
	rdfs:subPropertyOf	daq:hasMetric ;
	rdfs:comment	"Links Consistency Dimension with Obsolete Concepts In Ontology Metric" ;
	rdfs:label	"Understandability has obsolete concepts in ontology metric" ;
	rdfs:domain	dqm:Understandability ;
	rdfs:range	dqm:ObsoleteConceptsInOntologyMetric .	
	
dqm:ObsoleteConceptsInOntologyMetric
	a	rdfs:Class ;
	rdfs:subClassOf	daq:Metric ; 
		daq:expectedDataType xsd:double ;
	rdfs:comment	"Provides a measure for the number of classes and properties in an ontology which are marked as depricated. If an ontology is making lots of obsolete concepts between different versions, then this is an indicator that the ontology is going through a lot of changes, and is potentially in a state of poor quality" ;
	rdfs:label	"Obsolete concepts in ontology metric" .
		
#Synonym Usage in Ontology Classes
	dqm:hasSynonymUsageMetric
		a	rdfs:Property ;
		rdfs:subPropertyOf	daq:hasMetric ;
		rdfs:comment	"Links Accuracy Dimension with Synonym Usage Metric" ;
		rdfs:label	"Accuracy has synonym usage metric" ;
		rdfs:domain	dqm:Accuracy ;
		rdfs:range	dqm:SynonymUsageMetric .	
	
	dqm:SynonymUsageMetric
		a	rdfs:Class ;
		rdfs:subClassOf	daq:Metric ; 
		daq:expectedDataType xsd:double ;
		rdfs:comment	"Measures the number of classes which has a synonym <efo:alternative_term> described." ;
		rdfs:label	"Synonym usage metric" .
		
#POBO Definition Usage
	dqm:hasPOBODefinitionUsageMetric
		a	rdfs:Property ;
		rdfs:subPropertyOf	daq:hasMetric ;
		rdfs:comment	"Links Accuracy Dimension with POBO Definition Usage Metric" ;
		rdfs:label	"Accuracy has POBO definition usage metric" ;
		rdfs:domain	dqm:Accuracy ;
		rdfs:range	dqm:POBODefinitionUsageMetric .	
	
	dqm:POBODefinitionUsageMetric
		a	rdfs:Class ;
		rdfs:subClassOf	daq:Metric ; 
		daq:expectedDataType xsd:double ;
		rdfs:comment	"Provides a measure for an Ontology checking the usage of <pobo:def> in defined classes." ;
		rdfs:label	"POBO definition usage metric" .
		
	dqm:hasDefinedOntologyAuthorMetric
		a	rdfs:Property ;
		rdfs:subPropertyOf	daq:hasMetric ;
		rdfs:comment	"Links Accuracy Dimension with POBO Definition Usage Metric" ;
		rdfs:label	"Accuracy has defined ontology author metric" ;
		rdfs:domain	dqm:Accuracy ;
		rdfs:range	dqm:DefinedOntologyAuthorMetric .	
	
	dqm:DefinedOntologyAuthorMetric
		a	rdfs:Class ;
		rdfs:subClassOf	daq:Metric ; 
		daq:expectedDataType xsd:double ;
		rdfs:comment	"Checks whether the creator <efo:creator> is defined in the ontology." ;
		rdfs:label	"Defined ontology author" .
		
	dqm:HTTPSDataAccessMetric
		a	rdfs:Class ;
		rdfs:subClassOf	daq:Metric ; 
		daq:expectedDataType xsd:double ;
		rdfs:comment	"Verifies if access to the dataset is performed through a sound, HTTPS/SSL connection and thus, connection is confidential" ;
		rdfs:label	"Access to data through HTTPS metric" .
		
	dqm:hasHTTPSDataAccessMetric
		a	rdfs:Property ;
		rdfs:subPropertyOf	daq:hasMetric ;
		rdfs:comment	"Links security dimension with access to data through HTTPS metric" ;
		rdfs:label	"Security has access to data through HTTPS metric" ;
		rdfs:domain	dqm:Security ;
		rdfs:range	dqm:HTTPSDataAccessMetric .	
		
#Reputation
	
	dqm:OBOFoundryMetric
		a	rdfs:Class ;
		rdfs:subClassOf	daq:Metric ; 
		daq:expectedDataType xsd:double ;
		rdfs:comment "Detects non reputable resources by retrieving URI of resources from data sets and comparing them with URI found in reputable resources." ; 
		rdfs:label "OBO foundry metric" .
		
	dqm:hasOBOFoundryMetric
		a	rdfs:Property ;
		rdfs:subPropertyOf	daq:hasMetric ;
		rdfs:comment "Links Reputation category with OBO foundry metric" ; 
		rdfs:label "Reputation category has OBO foundry metric" ;
		rdfs:domain	dqm:Reputation ;
		rdfs:range	dqm:OBOFoundryMetric .


####################
#                  #
# Quality Problems #
#		   #
####################

## Specific classes and properties

### Dereferenceability
	
	dqm:SC200WithRDF
		a	rdfs:Class;
		rdfs:subClassOf qpro:Exception ;
		rdfs:comment "The described resource has a dereferenceability Status Code of 200 but returns an semantic content type" ;
		rdfs:label "200 OK Status Code with meaningful content type" .

	dqm:SC200WithoutRDF
		a	rdfs:Class;
		rdfs:subClassOf qpro:Exception ;
		rdfs:comment "The described resource has a dereferenceability Status Code of 200 but does not return a semantic content type" ;
		rdfs:label "200 OK Status Code without meaningful content type" .

	dqm:SC301MovedPermanently
		a	rdfs:Class;
		rdfs:subClassOf qpro:Exception ;
		rdfs:comment "The described resource has a dereferenceability Status Code of 301 Moved Permanently " ;
		rdfs:label "301 Moved Permanently" .

	dqm:SC302Found
		a	rdfs:Class;
		rdfs:subClassOf qpro:Exception ;
		rdfs:comment "The described resource has a dereferenceability Status Code of 302 Found" ;
		rdfs:label "302 Found" .

	dqm:SC307TemporaryRedirectory
		a	rdfs:Class;
		rdfs:subClassOf qpro:Exception ;
		rdfs:comment "The described resource has a dereferenceability Status Code of 307 Temporary Redirected" ;
		rdfs:label "307 Temporary Redirected" .

	dqm:SC3XXRedirection
		a	rdfs:Class;
		rdfs:subClassOf qpro:Exception ;
		rdfs:comment "The described resource has a dereferenceability Status Code of a 3XX Redirection but not the recommended 303 See Other" ;
		rdfs:label "3XX Redirection" .


	dqm:SC4XXClientError
		a	rdfs:Class;
		rdfs:subClassOf qpro:Exception ;
		rdfs:comment "The described resource has a dereferenceability Status Code of 4XX Client Error" ;
		rdfs:label "4XX Client Error" .


	dqm:SC5XXServerError
		a	rdfs:Class;
		rdfs:subClassOf qpro:Exception ;
		rdfs:comment "The described resource has a dereferenceability Status Code of 5XX Server Error" ;
		rdfs:label "5XX Server Error" .

	dqm:NotMeaningful
		a	rdfs:Class;
		rdfs:subClassOf qpro:Exception ;
		rdfs:comment "The described resource has a dereferenceable code as recommended by the LOD Principles (i.e. 303 See Other or Hash URI), but no meaningful data" ;
		rdfs:label "No Meaningful Data Returned" .

### RDF Accessibility

	dqm:NoRDFAccessibility
		a	rdfs:Class;
		rdfs:subClassOf qpro:Exception ;
		rdfs:comment "The dataset has no valid RDF Dump defined with the void:dataDump predicate" ;
		rdfs:label "RDF Dump Availablility" .

	dqm:InvalidDataDumpURI
		a	rdfs:Class;
		rdfs:subClassOf qpro:Exception ;
		rdfs:comment "The described URI is not a valid RDF data dump" ;
		rdfs:label "Invalid RDF Dump" .


### SPARQL EndPoint Accessibility
	dqm:NoEndPointAccessibility
		a	rdfs:Class;
		rdfs:subClassOf qpro:Exception ;
		rdfs:comment "The dataset has no valid SPARQL Endpoints defined with the void:sparqlEndpoint predicate" ;
		rdfs:label "SPARQL EndPoint Availablility" .

	dqm:InvalidSPARQLEndPoint
		a	rdfs:Class;
		rdfs:subClassOf qpro:Exception ;
		rdfs:comment "The described SPARQL endpoint is either invalid or not responding" ;
		rdfs:label "RDF Dump Availablility" .

### Misreported Content Type
	dqm:MisreportedTypeException
		a	rdfs:Class ;
		rdfs:subClassOf qpro:Exception ;
		rdfs:comment "The described Resource has a misreported content type"; 
		rdfs:label "Misreported Content Type" .

	dqm:expectedContentType
		a	rdfs:Property ;
		rdfs:subPropertyOf qpro:extraExceptionProperty ;
		rdfs:domain	rdfs:Resource ;
		rdfs:range	rdfs:Resource .

	dqm:actualContentType 
		a	rdfs:Property ;
		rdfs:subPropertyOf qpro:extraExceptionProperty ;
		rdfs:domain	rdfs:Resource ;
		rdfs:range	rdfs:Resource .

### Dereferenced Forward Links
	dqm:NotValidForwardLink
		a	rdfs:Class ;
		rdfs:subClassOf qpro:Exception ;
		rdfs:comment "The described resource do not resolve in a valid Dereferenced Forward-Link" ;
		rdfs:label "Not Valid Deferenceable Forward-Link" .

	dqm:ViolatingTriple
		a	rdfs:Class ;
		rdfs:subClassOf qpro:Exception ;
		rdfs:comment "The described resource has a violating forward link dereferencable triple" ;
		rdfs:label "Violating Triple" .

	dqm:hasViolatingTriple
		a rdfs:Property ;
		rdfs:subPropertyOf qpro:extraExceptionProperty ;
		rdfs:domain	rdfs:Resource ;
		rdfs:range	rdfs:Resource .


### Machine Readable Licence
	
	dqm:NoValidLicenceInDataset
		a	rdfs:Class ;
		rdfs:subClassOf qpro:Exception ;
		rdfs:comment "The described RDF Document/Dataset has no valid licence in the voID description or in its metadata" ;
		rdfs:label "No valid machine-readable licence" .
	

	dqm:NotRecommendedLicenceInDataset
		a	rdfs:Class ;
		rdfs:subClassOf qpro:Exception ;
		rdfs:comment "The described RDF Document/Dataset has a valid licence that is not recommended according to the voID W3C Standards" ;
		rdfs:label "Not Recommended machine-readable licence" .

### Machine Readable Licence
	
	dqm:NoValidLicenceInDatasetForHumans
		a	rdfs:Class ;
		rdfs:subClassOf qpro:Exception ;
		rdfs:comment "The described RDF Document/Dataset has no valid licence in the in its descriptive metadata" ;
		rdfs:label "No valid human-readable licence" .
	

	dqm:NotRecommendedLicenceInDatasetForHumans
		a	rdfs:Class ;
		rdfs:subClassOf qpro:Exception ;
		rdfs:comment "The described RDF Document/Dataset has a valid licence that is not recommended according to the voID W3C Standards" ;
		rdfs:label "Not Recommended human-readable licence" .

## Correct URI Usage

	dqm:IncorrectCoolURIUsage
		a	rdfs:Class ;
		rdfs:subClassOf qpro:Exception ;
		rdfs:comment "An Incorrect URI style used for dataset. For datasets with more than 500K triples Slash URIs are suggested, whilst for less than 500K triples Hash URIs should be used" ;
		rdfs:label "Incorrect Usage of URIs" .


### Dereferenced Back Links
	dqm:NotValidDereferenceableBackLink
		a	rdfs:Class ;
		rdfs:subClassOf qpro:Exception ;
		rdfs:comment "The described resource do not resolve in a valid Dereferenced Link" ;
		rdfs:label "Not Valid Deferenceable Backlink" .

	dqm:NoBackLink
		a	rdfs:Class ;
		rdfs:subClassOf qpro:Exception ;
		rdfs:comment "The described resource does not provide a valid back link" ;
		rdfs:label "No Backlink" .

	dqm:hasNoBackLink
		a rdfs:Property ;
		rdfs:subPropertyOf qpro:extraExceptionProperty ;
		rdfs:domain	rdfs:Resource ;
		rdfs:range	rdfs:Resource .


### Links To External Data Providers

	dqm:NoValidRDFDataForExternalLink
		a	rdfs:Class ;
		rdfs:subClassOf qpro:Exception ;
		rdfs:comment "The External Link provided does not give valid RDF" ;
		rdfs:label "No valid RDF for External Link" .

	dqm:LowPercentageOfValidPLDResources
		a	rdfs:Class ;
		rdfs:subClassOf qpro:Exception ;
		rdfs:comment "The External Link provide a low number of resources that provide RDF" ;
		rdfs:label "Low Percentage of valid RDF resources in PLD" .


### Short URIs
	
	dqm:ParametarisedURI
		a	rdfs:Class ;
		rdfs:subClassOf qpro:Exception ;
		rdfs:comment "The resource URI includes a parameterised string." ;
		rdfs:label "Parametarised URI" .

	dqm:LongURI
		a	rdfs:Class ;
		rdfs:subClassOf qpro:Exception ;
		rdfs:comment "According to W3C URI standards, a URI should not be longer than 80 characters including the schema. Long URIs are not recommended. Refer to CoolURIs (http://www.linkeddata.org/how-to-publish)" ;
		rdfs:label "Long URI Exception" .


### No Prolix RDF

	dqm:UsageOfReification
		a	rdfs:Class ;
		rdfs:subClassOf qpro:Exception ;
		rdfs:comment "The resource is using RDF reification feature (type - rdf:Statement). The use of rdf:Statement or any other prolix feature is strongly discouraged." ;
		rdfs:label "Usage of Reification in Dataset" .

	dqm:UsageOfContainers
		a	rdfs:Class ;
		rdfs:subClassOf qpro:Exception ;
		rdfs:comment "The resource is using RDF containers feature (type - rdf:Container). The use of rdf:Container or any other prolix feature is strongly discouraged." ;
		rdfs:label "Usage of Containers in Dataset" .


	dqm:UsageOfCollections
		a	rdfs:Class ;
		rdfs:subClassOf qpro:Exception ;
		rdfs:comment "The resource is using RDF collections feature. The use of rdf:Alt, rdf:Bag, rdf:List, or any other prolix feature is strongly discouraged." ;
		rdfs:label "Usage of Collections" .


### DifferentSerialisationsMetric
	dqm:NoMultipleFormatDefined
		a	rdfs:Class ;
		rdfs:subClassOf qpro:Exception ;
		rdfs:comment "The dataset must have more than one serialisation format defined using the void:feature predicate." ;
		rdfs:label "No format defined for a dataset" .

	dqm:IncorrectFormatDefined
		a	rdfs:Class ;
		rdfs:subClassOf qpro:Exception ;
		rdfs:comment "The defined format using the void:feature predicate is unknown. Check http://www.w3.org/ns/formats/." ;
		rdfs:label "Incorrect defined format/feature" .

### Undefined Classes and Properties
	
	dqm:UndefinedClass
		a	rdfs:Class ;
		rdfs:subClassOf qpro:Exception ;
		rdfs:comment "The class used is undefined in the respective schema" ;
		rdfs:label "Undefined Class" .

	dqm:UndefinedProperty
		a	rdfs:Class ;
		rdfs:subClassOf qpro:Exception ;
		rdfs:comment "The property used is undefined in its respective schema." ;
		rdfs:label "Undefined Property" .


### Reuse of Terms and Vocabularies

	dqm:UnusedSuggestedVocabulary
		a	rdfs:Class ;
		rdfs:subClassOf qpro:Exception ;
		rdfs:comment "The dataset did not use terms from the suggested vocabulary." ;
		rdfs:label "Unused suggested vocabulary" .


### Entities members of disjoint classes
	
	dqm:MultiTypedResourceWithDisjointedClasses
		a	rdfs:Class ;
		rdfs:subClassOf qpro:Exception ;
		rdfs:comment "The referred resource is multi-typed with disjoined classes." ;
		rdfs:label "Disjoined Classes Typing" .

	dqm:violatingDisjoinedClass
		a rdfs:Property ;
		rdfs:subPropertyOf qpro:extraExceptionProperty ;
		rdfs:domain	rdfs:Resource;
		rdfs:range	rdfs:Resource .


### Entities members of disjoint classes
	
	dqm:MisplacedClass
		a	rdfs:Class ;
		rdfs:subClassOf qpro:Exception ;
		rdfs:comment "The referred resource used a defined class instead of a property." ;
		rdfs:label "Misplaced Class" .

	dqm:hasMisplacedClass
		a rdfs:Property ;
		rdfs:subPropertyOf qpro:extraExceptionProperty ;
		rdfs:domain	rdfs:Resource;
		rdfs:range	rdfs:Resource .


	dqm:MisplacedProperty
		a	rdfs:Class ;
		rdfs:subClassOf qpro:Exception ;
		rdfs:comment "The referred resource used a defined property instead of a class." ;
		rdfs:label "Misplaced Property" .

	dqm:hasMisplacedProperty
		a rdfs:Property ;
		rdfs:subPropertyOf qpro:extraExceptionProperty ;
		rdfs:domain	rdfs:Resource;
		rdfs:range	rdfs:Resource .


### Misuse of owl:DatatypeProperty or owl:ObjectProprty	
	dqm:MisusedDatatypeProperty
		a	rdfs:Class ;
		rdfs:subClassOf qpro:Exception ;
		rdfs:comment "The referred resource used a datatype property instead of an Object Property." ;
		rdfs:label "Misused Datatype Property" .

	dqm:hasMisusedDatatypeProperty
		a rdfs:Property ;
		rdfs:subPropertyOf qpro:extraExceptionProperty ;
		rdfs:domain	rdfs:Resource;
		rdfs:range	rdfs:Resource .


	dqm:MisusedObjectProperty
		a	rdfs:Class ;
		rdfs:subClassOf qpro:Exception ;
		rdfs:comment "The referred resource used an object property instead of a datatype property." ;
		rdfs:label "Misplaced Property" .

	dqm:hasMisusedObjectProperty
		a rdfs:Property ;
		rdfs:subPropertyOf qpro:extraExceptionProperty ;
		rdfs:domain	rdfs:Resource;
		rdfs:range	rdfs:Resource .


### CurrencyOfDataset
	dqm:MissingMetadataForCurrency
		a	rdfs:Class ;
		rdfs:subClassOf qpro:Exception ;
		rdfs:comment "The referred dataset have missing metadata properties thus cannot calculate currency." ;
		rdfs:label "Missing Metadata for Currency Calculation" .

	dqm:MissingMetadataForFreshness
		a	rdfs:Class ;
		rdfs:subClassOf qpro:Exception ;
		rdfs:comment "The referred dataset have missing metadata properties thus cannot calculate data freshness." ;
		rdfs:label "Missing Metadata for Freshness Calculation" .

	dqm:MissingMetadataForTimelinessOfResource
		a	rdfs:Class ;
		rdfs:subClassOf qpro:Exception ;
		rdfs:comment "The referred dataset have missing metadata properties thus cannot calculate data timeliness." ;
		rdfs:label "Missing Metadata for  Calculation" .

### Extensional Conciseness
	dqm:ResourceReplica
		a	rdfs:Class ;
		rdfs:subClassOf qpro:Exception ;
		rdfs:comment "The referred resource has a replica resource with a different id." ;
		rdfs:label "Resource Replica" .
